proof/correctness/avx2/Kyber_AVX_AuxLemmas.ec
@@ -1,0 +1,151 @@
+require import AllCore List Int IntDiv CoreMap Real Number.
+from Jasmin require import JModel.
+require import Array400 Array384 Array256 Array128 Array64 Array32 Array16 Array4 Array8 Array2.
+require import W16extra WArray512 WArray32 WArray16.
+require import AVX2_Ops.
+require import KyberPoly.
+require import KyberINDCPA.
+import Kyber.
+import KyberPoly.
+import Zq.
+
+op lift2poly (p: W256.t): W16.t Array16.t =
+  Array16.init (fun (n : int) => p \bits16 n).
+
+op f16u16_t8u32 (t: t16u16): t8u32 = Array8.init (fun i => pack2_t (W2u16.Pack.init (fun j => t.[2*i + j]))).
+op f8u32_t16u16 (t: t8u32): t16u16 = Array16.init (fun i => t.[i %/ 2] \bits16 (i %% 2)).
+
+op f32u8_t16u16 (t: t32u8): t16u16 = Array16.init (fun i => pack2_t (W2u8.Pack.init (fun j => t.[2*i + j]))).
+op f16u16_t32u8 (t: t16u16): t32u8 = Array32.init (fun i => t.[i %/ 2] \bits8 (i %% 2)).
+
+op f8u32_t4u64 (t: t8u32): t4u64 = Array4.init (fun i => pack2_t (W2u32.Pack.init (fun j => t.[2*i + j]))).
+op f4u64_t8u32 (t: t4u64): t8u32 = Array8.init (fun i => t.[i %/ 2] \bits32 (i %% 2)).
+
+op f32u8_t4u64 (t: t32u8): t4u64 = Array4.init (fun i => pack8_t (W8u8.Pack.init (fun j => t.[8*i + j]))).
+op f4u64_t32u8 (t: t4u64): t32u8 = Array32.init (fun i => t.[i %/ 8] \bits8 (i %% 8)).
+
+op f32u8_t8u32 (t: t32u8): t8u32 = Array8.init (fun i => pack4_t (W4u8.Pack.init (fun j => t.[4*i + j]))).
+op f8u32_t32u8 (t: t8u32): t32u8 = Array32.init (fun i => t.[i %/ 4] \bits8 (i %% 4)).
+
+op f16u16_t4u64 (t: t16u16): t4u64 = Array4.init (fun i => pack4_t (W4u16.Pack.init (fun j => t.[4*i + j]))).
+op f4u64_t16u16 (t: t4u64): t16u16 = Array16.init (fun i => t.[i %/ 4] \bits16 (i %% 4)).
+
+op f4u64_t2u128 (t: t4u64): t2u128 = Array2.init (fun i => pack2_t (W2u64.Pack.init (fun j => t.[2*i + j]))).
+op f2u128_t4u64 (t: t2u128): t4u64 = Array4.init (fun i => t.[i %/ 2] \bits64 (i %% 2)).
+
+op f16u16_t2u128 (t: t16u16): t2u128 = Array2.init (fun i => pack8_t (W8u16.Pack.init (fun j => t.[8*i + j]))).
+op f2u128_t16u16 (t: t2u128): t16u16 = Array16.init (fun i => t.[i %/ 8] \bits16 (i %% 8)).
+
+lemma lift2poly_iso (p: W16.t Array256.t) (i k: int):
+    0 <= i < 16 =>
+    16 * i <= k < 16 * i + 16 => (lift2poly (get256 (WArray512.init16 (fun j => p.[j])) i)).[k %% 16] = p.[k].
+proof. 
+  move => i_b k_b.
+  have k_mb: 0 <= k %% 16 < 16.
+    smt(@IntDiv).
+  rewrite /x.
+  rewrite /lift2poly initiE => />.
+  rewrite get256E => />.
+  rewrite k_mb //=.
+  rewrite initiE. move : k_mb => /#.
+  rewrite initiE. move : k_mb => /#.
+  simplify.
+  rewrite /init16.
+  rewrite initiE. move : k_mb => /#.
+  rewrite initiE. move : k_mb => /#.
+  simplify.
+  rewrite (_: (32 * i + (2 * (k %% 16) + 1)) %/ 2 = (32 * i + 2 * (k %% 16)) %/ 2).
+    smt(@IntDiv).
+  rewrite (_: (32 * i + 2 * (k %% 16)) %% 2 = 0).
+    smt(@IntDiv).
+  rewrite (_: (32 * i + (2 * (k %% 16) + 1)) %% 2 = 1).
+    smt(@IntDiv).
+  rewrite pack2_bits8.
+  smt(@IntDiv).
+qed.
+
+lemma set_get_def (v : W16.t Array256.t) (w: W256.t) i j :
+    0 <= i < 16 => 0 <= j < 256 =>
+    WArray512.get16
+    (WArray512.set256 (WArray512.init16 (fun i => v.[i])) i w) j =
+      if 16 * i <= j < 16 * i + 16 then w \bits16 (j %% 16)
+      else v.[j].
+proof. 
+  move => hx hs; rewrite set256E !get16E.
+  rewrite -(W2u8.unpack8K (if 16 * i <= j < 16 * i + 16 then w \bits16 (j %% 16) else v.[j])); congr.
+  apply W2u8.Pack.ext_eq => k hk.
+  rewrite W2u8.get_unpack8 //= W2u8.Pack.initiE 1:/# /=.
+  rewrite initiE /=. move : hk hs => /#.
+  rewrite initiE /=. move : hk hs => /#.
+  have ->: (32 * i <= 2 * j + k < 32 * i + 32) = (16 * i <= j < 16 * i + 16) by smt().
+  case : (16 * i <= j < 16 * i + 16) => h.
+    + by rewrite W256_bits16_bits8 1:// /#.
+    + by rewrite /init16 /#.
+qed.
+
+lemma set_get_eq (v: W16.t Array256.t) (w: W256.t) i j:
+    0 <= i < 16 => 0 <= j < 256 => 16 * i <= j < 16 * i + 16 =>
+    WArray512.get16
+    (WArray512.set256 (WArray512.init16 (fun i => v.[i])) i w) j =
+      w \bits16 j %% 16.
+proof. 
+  by move => h1 h2 h3; rewrite set_get_def // h3.
+qed.
+
+lemma set_get_diff (v: W16.t Array256.t) (w: W256.t) i j:
+    0 <= i < 16 => 0 <= j < 256 => !(16 * i <= j < 16 * i + 16) =>
+    WArray512.get16
+    (WArray512.set256 (WArray512.init16 (fun i => v.[i])) i w) j =
+      v.[j].
+proof.
+  move => h1 h2 h3; rewrite set_get_def // h3. auto.
+qed.
+
+lemma get_set_get_eqb (v: W16.t Array256.t) (w: W256.t) i:
+  0 <= i < 16 => forall k, 0 <= k < i*16 =>
+  v.[k] = (Array256.init (WArray512.get16 (WArray512.set256 (WArray512.init16 (fun j => v.[j])) i w))).[k].
+proof. 
+  move => i_i k k_i.
+  rewrite Array256.initiE.
+  move : i_i k_i. smt().
+  simplify.
+  rewrite set_get_def => /#.
+qed.
+
+lemma get_set_get_eqa (v: W16.t Array256.t) (w: W256.t) i:
+  0 <= i < 16 => forall k, i*16 + 16 <= k < 256 =>
+  v.[k] = (Array256.init (WArray512.get16 (WArray512.set256 (WArray512.init16 (fun j => v.[j])) i w))).[k].
+proof.
+  move => i_i k k_i.
+  rewrite Array256.initiE.
+  move : i_i k_i => /#.
+  simplify.
+  rewrite set_get_def => /#.
+qed.
+
+lemma get_set_get_diff (v: W16.t Array256.t) (w: vt16u16) i:
+  0 <= i < 16 => forall k, i*16 <= k < i*16 + 16 =>
+  w \bits16 (k%%16) = (Array256.init (WArray512.get16 (WArray512.set256 (WArray512.init16 (fun j => v.[j])) i w))).[k].
+proof. 
+  move => i_i k k_i.
+  rewrite Array256.initiE.
+  move : i_i k_i => /#.
+  simplify.
+  rewrite set_get_def => /#.
+qed.
+
+lemma get_lift_array256_eq (p: W16.t Array256.t):
+  let p_lift = lift_array256 p in
+  forall k, 0 <= k < 256 => p_lift.[k] = inFq (W16.to_sint p.[k]).
+proof. 
+  rewrite /lift_array256 => p_lift. rewrite /p_lift.
+  move => k k_i.
+  smt (@Array256).
+qed.
+
+lemma lift_array256E (x : W16.t Array256.t) k :
+  0 <= k < 256 =>
+  (lift_array256 x).[k] = inFq (to_sint x.[k]).
+proof. 
+by move => ?; rewrite /lift_array256 mapiE //. 
+qed.
